books/centaur/gl/eval-g-base-help.lisp
@@ -16,20 +16,24 @@
 (acl2::def-functional-instance
  eval-g-base-alt-def
  generic-geval-alt-def
- ((apply-stub eval-g-base-apply)
-  (generic-geval-apply eval-g-base-apply)
+ ((generic-geval-ev eval-g-base-ev)
+  (generic-geval-ev-lst eval-g-base-ev-lst)
   (generic-geval eval-g-base))
- :hints ('(:do-not-induct
-           t
+ :hints ('(:in-theory (e/d* (eval-g-base-ev-constraint-0
+                             eval-g-base-apply-agrees-with-eval-g-base-ev)
+                            (eval-g-base-apply))
            :expand ((eval-g-base x env))))
+         ;; :do-not-induct
+         ;;   t
+         ;;   :expand ((eval-g-base x env))))
  :rule-classes ((:definition :clique (eval-g-base))))
 
 
 (acl2::def-functional-instance
  mk-g-boolean-correct-for-eval-g-base
  mk-g-boolean-correct
- ((apply-stub eval-g-base-apply)
-  (generic-geval-apply eval-g-base-apply)
+ ((generic-geval-ev eval-g-base-ev)
+  (generic-geval-ev-lst eval-g-base-ev-lst)
   (generic-geval eval-g-base)))
 
 
@@ -37,15 +41,15 @@
 (acl2::def-functional-instance
  gtests-obj-correct-for-eval-g-base
  gtests-obj-correct
- ((apply-stub eval-g-base-apply)
-  (generic-geval-apply eval-g-base-apply)
+ ((generic-geval-ev eval-g-base-ev)
+  (generic-geval-ev-lst eval-g-base-ev-lst)
   (generic-geval eval-g-base)))
 
 (acl2::def-functional-instance
  gtests-nonnil-correct-for-eval-g-base
  gtests-nonnil-correct
- ((apply-stub eval-g-base-apply)
-  (generic-geval-apply eval-g-base-apply)
+ ((generic-geval-ev eval-g-base-ev)
+  (generic-geval-ev-lst eval-g-base-ev-lst)
   (generic-geval eval-g-base)))
 
 (local
@@ -56,37 +60,37 @@
    (acl2::def-functional-instance
     mk-g-ite-correct-for-eval-g-base
     mk-g-ite-correct
-    ((apply-stub eval-g-base-apply)
-     (generic-geval-apply eval-g-base-apply)
+    ((generic-geval-ev eval-g-base-ev)
+     (generic-geval-ev-lst eval-g-base-ev-lst)
      (generic-geval eval-g-base)))
 
 
    (acl2::def-functional-instance
     gobj-ite-merge-correct-for-eval-g-base
     gobj-ite-merge-correct
-    ((apply-stub eval-g-base-apply)
-     (generic-geval-apply eval-g-base-apply)
+    ((generic-geval-ev eval-g-base-ev)
+     (generic-geval-ev-lst eval-g-base-ev-lst)
      (generic-geval eval-g-base)))))
 
 (acl2::def-functional-instance
  eval-g-base-g-apply
  generic-geval-g-apply
- ((apply-stub eval-g-base-apply)
-  (generic-geval-apply eval-g-base-apply)
+ ((generic-geval-ev eval-g-base-ev)
+  (generic-geval-ev-lst eval-g-base-ev-lst)
   (generic-geval eval-g-base)))
 
 (acl2::def-functional-instance
  general-consp-car-correct-for-eval-g-base
  general-consp-car-correct
- ((apply-stub eval-g-base-apply)
-  (generic-geval-apply eval-g-base-apply)
+ ((generic-geval-ev eval-g-base-ev)
+  (generic-geval-ev-lst eval-g-base-ev-lst)
   (generic-geval eval-g-base)))
 
 (acl2::def-functional-instance
  general-consp-cdr-correct-for-eval-g-base
  general-consp-cdr-correct
- ((apply-stub eval-g-base-apply)
-  (generic-geval-apply eval-g-base-apply)
+ ((generic-geval-ev eval-g-base-ev)
+  (generic-geval-ev-lst eval-g-base-ev-lst)
   (generic-geval eval-g-base)))
 
 (in-theory (disable general-consp-car-correct-for-eval-g-base
@@ -95,15 +99,15 @@
 (acl2::def-functional-instance
  eval-g-base-cons
  generic-geval-cons
- ((apply-stub eval-g-base-apply)
-  (generic-geval-apply eval-g-base-apply)
+ ((generic-geval-ev eval-g-base-ev)
+  (generic-geval-ev-lst eval-g-base-ev-lst)
   (generic-geval eval-g-base)))
 
 (acl2::def-functional-instance
  eval-g-base-non-cons
  generic-geval-non-cons
- ((apply-stub eval-g-base-apply)
-  (generic-geval-apply eval-g-base-apply)
+ ((generic-geval-ev eval-g-base-ev)
+  (generic-geval-ev-lst eval-g-base-ev-lst)
   (generic-geval eval-g-base)))
 
 (in-theory (disable eval-g-base-non-cons))
@@ -118,43 +122,43 @@
 (acl2::def-functional-instance
  general-concrete-obj-when-consp-for-eval-g-base
  general-concrete-obj-when-consp
- ((apply-stub eval-g-base-apply)
-  (generic-geval-apply eval-g-base-apply)
+ ((generic-geval-ev eval-g-base-ev)
+  (generic-geval-ev-lst eval-g-base-ev-lst)
   (generic-geval eval-g-base)))
 
 (acl2::def-functional-instance
  not-general-numberp-not-acl2-numberp-for-eval-g-base
  not-general-numberp-not-acl2-numberp
- ((apply-stub eval-g-base-apply)
-  (generic-geval-apply eval-g-base-apply)
+ ((generic-geval-ev eval-g-base-ev)
+  (generic-geval-ev-lst eval-g-base-ev-lst)
   (generic-geval eval-g-base)))
 
 (acl2::def-functional-instance
  mk-g-number-correct-for-eval-g-base
  mk-g-number-correct
- ((apply-stub eval-g-base-apply)
-  (generic-geval-apply eval-g-base-apply)
+ ((generic-geval-ev eval-g-base-ev)
+  (generic-geval-ev-lst eval-g-base-ev-lst)
   (generic-geval eval-g-base)))
 
 (acl2::def-functional-instance
  mk-g-concrete-correct-for-eval-g-base
  mk-g-concrete-correct
- ((apply-stub eval-g-base-apply)
-  (generic-geval-apply eval-g-base-apply)
+ ((generic-geval-ev eval-g-base-ev)
+  (generic-geval-ev-lst eval-g-base-ev-lst)
   (generic-geval eval-g-base)))
 
 (acl2::def-functional-instance
  g-concrete-quote-correct-for-eval-g-base
  g-concrete-quote-correct
- ((apply-stub eval-g-base-apply)
-  (generic-geval-apply eval-g-base-apply)
+ ((generic-geval-ev eval-g-base-ev)
+  (generic-geval-ev-lst eval-g-base-ev-lst)
   (generic-geval eval-g-base)))
 
 (acl2::def-functional-instance
  eval-g-base-of-gl-cons
  generic-geval-gl-cons
- ((apply-stub eval-g-base-apply)
-  (generic-geval-apply eval-g-base-apply)
+ ((generic-geval-ev eval-g-base-ev)
+  (generic-geval-ev-lst eval-g-base-ev-lst)
   (generic-geval eval-g-base)))
 
 
