books/centaur/gl/g-intern.lisp
@@ -68,11 +68,13 @@
    (acl2::def-functional-instance
     mk-g-ite-correct-for-eval-g-base
     mk-g-ite-correct
-    ((apply-stub eval-g-base-apply)
-     (generic-geval-apply eval-g-base-apply)
+    ((generic-geval-ev eval-g-base-ev)
+     (generic-geval-ev-lst eval-g-base-ev-lst)
      (generic-geval eval-g-base))
-    :hints((and stable-under-simplificationp
-                '(:expand ((:with eval-g-base (eval-g-base x env)))))))))
+ :hints ('(:in-theory (e/d* (eval-g-base-ev-constraint-0
+                             eval-g-base-apply-agrees-with-eval-g-base-ev)
+                            (eval-g-base-apply))
+           :expand ((:with eval-g-base (eval-g-base x env))))))))
 
 
 (def-g-correct-thm intern-in-package-of-symbol eval-g-base
@@ -88,4 +90,3 @@
                                   (eval-g-base acl2::sym env))
                            (:with eval-g-base
                                   (eval-g-base acl2::str env)))))))
-
