books/centaur/gl/generic-geval.lisp
@@ -6,9 +6,10 @@
 (include-book "bvecs")
 (include-book "tools/bstar" :dir :system)
 (include-book "tools/templates" :dir :system)
-(include-book "defapply")
-(include-book "defapply-proofs")
+;; (include-book "defapply")
+;; (include-book "defapply-proofs")
 (include-book "cutil/defmvtypes" :dir :system)
+(include-book "../misc/defapply")
 
 (defun acl2::boolfix (x)
   (declare (xargs :guard t))
@@ -126,9 +127,11 @@
            (eqlable-alistp x)))
 
 
+
 (defconst *geval-template*
   '(progn
-     (defapply _geval_-apply _apply-fns_)
+     (acl2::defapply/ev/concrete-ev _geval_ _apply-fns_)
+     ;; (defapply _geval_-apply _apply-fns_)
      (defun _geval_ (x env)
        (declare (xargs :guard (consp env)
                        :measure (acl2-count x)
@@ -172,8 +175,15 @@
               (_geval_ else env)))
 
            ;; Apply: Unevaluated function call.
-           ((g-apply fn args) (_geval_-apply fn (_geval_ args env)))
-
+           ((g-apply fn args)
+            (let* ((args (_geval_ args env)))
+              (mbe :logic (_geval_-ev (cons fn (kwote-lst args)) nil)
+                   :exec (b* ((args (acl2::list-fix args))
+                              ((mv ok val) (_geval_-apply fn args))
+                              ((when ok) val))
+                           (_geval_-ev (cons fn (kwote-lst args))
+                                       nil)))))
+ 
            ;; Var: untyped variable.
            ((g-var name)   (cdr (het name (cdr env))))
 
@@ -186,13 +196,14 @@
                        :measure (acl2-count x)
                        :guard-hints (("goal" :in-theory
                                       '((:type-prescription v2i)
+                                        (alistp)
                                         (:type-prescription v2n)
                                         (:type-prescription hons-assoc-equal)
                                         hons-get
+                                        acl2::true-listp-of-list-fix
                                         acl2::assoc-eql-exec-is-assoc-equal
                                         eqlablep-compound-recognizer
                                         consp-assoc-equal-of-cons
-                                        _geval_-apply-arities
                                         symbol-alistp-implies-eqlable-alistp)))
                        :hints (("goal" :in-theory '(measure-for-geval atom)))))
        (if (atom x)
@@ -234,12 +245,8 @@
 
            ;; Apply: Unevaluated function call.
            ((g-apply fn args)
-            (let* ((args (_geval_-appalist args env appal))
-                   (look (member-equal (cons fn (len args))
-                                       (_geval_-apply-arities))))
-              (if (and look (true-listp args))
-                  (_geval_-apply fn args)
-                (cdr (assoc (cons fn args) appal)))))
+            (let* ((args (_geval_-appalist args env appal)))
+              (ec-call (_geval_-ev-concrete (cons fn (kwote-lst (acl2::list-fix args))) nil appal))))
 
            ;; Var: untyped variable.
            ((g-var name)   (cdr (het name (cdr env))))
@@ -248,7 +255,12 @@
            (& (cons (_geval_-appalist (car x) env appal)
                     (_geval_-appalist (cdr x) env appal))))))
      
-     (table eval-g-table '_geval_ '(_geval_-appalist _geval_-apply _geval_-apply-arities))))
+     (table eval-g-table '_geval_ '(_geval_-appalist
+                                    _geval_-ev
+                                    _geval_-ev-lst
+                                    _geval_-ev-concrete
+                                    _geval_-ev-concrete-lst
+                                    . _apply-fns_))))
 
 
 (defun def-geval-fn (geval fns)
@@ -266,6 +278,115 @@
 
 (def-geval generic-geval nil)
 
+;; (defthm generic-geval-apply-ev-lst-of-kwote-lst
+;;   (equal (generic-geval-apply-ev-lst (kwote-lst x) a)
+;;          (acl2::list-fix x)))
+
+;; ;; (defthm generic-geval-apply-ev-lst-of-kwote-lst-a
+;; ;;   (implies (syntaxp (not (equal a ''nil)))
+;; ;;            (equal (generic-geval-apply-ev-lst (kwote-lst x) a)
+;; ;;                   (generic-geval-apply-ev-lst (kwote-lst x) nil))))
+
+;; ;; (defthm kwote-lst-of-generic-geval-apply-ev-lst-of-kwote-lst
+;; ;;   (equal (kwote-lst (generic-geval-apply-ev-lst (kwote-lst x) a))
+;; ;;          (kwote-lst x)))
+
+;; (defthm true-listp-generic-geval-apply-ev-lst
+;;   (true-listp (generic-geval-apply-ev-lst x a))
+;;   :hints (("Goal" :induct (len x))))
+
+;; (mutual-recursion
+;;  (defund generic-geval-apply-ev-substitution (x a appalist)
+;;    (cond ((atom x) (and x (cdr (assoc x a))))
+;;          ((eq (car x) 'quote) (cadr x))
+;;          ((consp (car x))
+;;           (generic-geval-apply-ev-substitution
+;;            (caddar x)
+;;            (pairlis$ (cadar x)
+;;                      (generic-geval-apply-ev-substitution-lst
+;;                       (cdr x) a appalist))
+;;            appalist))
+;;          ((assoc (car x) (generic-geval-apply-arities))
+;;           (generic-geval-apply-ev (cons (car x)
+;;                                         (kwote-lst
+;;                                          (generic-geval-apply-ev-substitution-lst
+;;                                           (cdr x) a appalist)))
+;;                                   nil))
+;;          (t (cdr (assoc (cons (car x)
+;;                               (generic-geval-apply-ev-substitution-lst
+;;                                (cdr x) a appalist))
+;;                         appalist)))))
+
+;;  (defund generic-geval-apply-ev-substitution-lst (x a appalist)
+;;    (if (atom x)
+;;        nil
+;;      (cons (generic-geval-apply-ev-substitution (car x) a appalist)
+;;            (generic-geval-apply-ev-substitution-lst (cdr x) a appalist)))))
+
+
+;; (defun list-equiv1 (x y)
+;;   (if (and (atom x) (atom y))
+;;       t
+;;     (and (consp x) (consp y)
+;;          (equal (car x) (car y))
+;;          (list-equiv1 (cdr x) (cdr y)))))
+
+;; (defthmd list-equiv-is-list-equiv1
+;;   (equal (acl2::list-equiv x y)
+;;          (list-equiv1 x y)))
+
+;; (defcong acl2::list-equiv equal (generic-geval-apply-ev-lst x a) 1
+;;   :hints (("goal" ::in-theory (enable list-equiv-is-list-equiv1))))
+
+;; (defcong acl2::list-equiv equal (generic-geval-apply-ev-substitution-lst x a appalist) 1
+;;   :hints (("goal" ::in-theory (enable list-equiv-is-list-equiv1)
+;;            :induct (list-equiv1 x acl2::x-equiv)
+;;            :expand ((generic-geval-apply-ev-substitution-lst
+;;                      x a appalist)
+;;                     (generic-geval-apply-ev-substitution-lst
+;;                      acl2::x-equiv a appalist)))))
+
+;; (defcong acl2::list-equiv equal (kwote-lst x) 1
+;;   :hints (("goal" ::in-theory (enable list-equiv-is-list-equiv1))))
+
+;; (defcong acl2::list-equiv equal (generic-geval-apply f args) 2
+;;   :hints(("Goal" :in-theory (enable generic-geval-apply))))
+
+;; (defthm generic-geval-apply-ev-substitution-lst-of-kwote-lst
+;;   (equal (generic-geval-apply-ev-substitution-lst (kwote-lst x) a appalist)
+;;          (acl2::list-fix x))
+;;   :hints (("goal" :induct (kwote-lst x)
+;;            :expand ((:free (x y)
+;;                      (generic-geval-apply-ev-substitution-lst
+;;                       (cons x y) a appalist))
+;;                     (generic-geval-apply-ev-substitution-lst
+;;                      nil a appalist)
+;;                     (generic-geval-apply-ev-substitution
+;;                      (list 'quote (car x)) a appalist)))))
+
+;; (defthm sdfasd
+;;   t
+;;   :hints (("goal" :use
+;;            ((:functional-instance
+;;              (:theorem (equal (generic-geval-apply-ev-substitution x a appalist)
+;;                               (generic-geval-apply-ev-substitution x a appalist)))
+;;              (generic-geval-apply-ev-lst
+;;               (lambda (x a)
+;;                 (generic-geval-apply-ev-substitution-lst x a appalist)))
+;;              (generic-geval-apply-ev
+;;               (lambda (x a)
+;;                 (generic-geval-apply-ev-substitution x a appalist)))))
+;;            :expand ((generic-geval-apply-ev-substitution x a appalist))
+;;            :in-theory (enable
+;;                        generic-geval-apply
+;;                        generic-geval-apply-ev-substitution
+;;                        generic-geval-apply-ev-substitution-lst)
+;;            :do-not-induct t))
+;;   :rule-classes nil
+;;   :otf-flg t)
+                     
+           
+
 (local (defthm generic-geval-appalist-is-instance-of-generic-geval
          t
          :hints (("goal" :use ((:functional-instance
@@ -273,23 +394,41 @@
                                 (generic-geval
                                  (lambda (x env)
                                    (generic-geval-appalist x env appalist)))
-                                (apply-stub
-                                 (lambda (f args)
-                                   (cdr (assoc (cons f args) appalist))))
-                                (generic-geval-apply
-                                 (lambda (fn args)
-                                   (LET*
-                                    ((LOOK (MEMBER-EQUAL (CONS FN (LEN ARGS))
-                                                         (GENERIC-GEVAL-APPLY-ARITIES))))
-                                    (IF (AND LOOK (TRUE-LISTP ARGS))
-                                        (GENERIC-GEVAL-APPLY FN ARGS)
-                                        (CDR (ASSOC (CONS FN ARGS)
-                                                    APPALIST))))))))
-                  :in-theory '(generic-geval-apply
-                               generic-geval-apply-arities
-                               member-equal
-                               generic-geval-appalist)))
-         :rule-classes nil))
+                                (generic-geval-ev
+                                 (lambda (x a)
+                                   (generic-geval-ev-concrete x a appalist)))
+                                (generic-geval-ev-lst
+                                 (lambda (x a)
+                                   (generic-geval-ev-concrete-lst
+                                    x a appalist)))))
+                  ;; '(generic-geval-apply-ev-lst-of-atom
+                             ;;   generic-geval-apply-ev-substitution)
+                  ;; :in-theory '(generic-geval-apply
+                  ;;              generic-geval-apply-arities
+                  ;;              member-equal
+                  ;;              generic-geval-appalist)
+                  :do-not-induct t)
+                 ;; (and stable-under-simplificationp
+                 ;;      '(:in-theory (enable
+                 ;;                    generic-geval-apply-ev-of-fncall-args)
+                 ;;        :expand ((:free (a)
+                 ;;                  (generic-geval-apply-ev-substitution
+                 ;;                   x a appalist))
+                 ;;                 (:free (x y a)
+                 ;;                  (generic-geval-apply-ev-substitution
+                 ;;                   (cons x y) a appalist)))))
+                 ;; (and stable-under-simplificationp
+                 ;;      '(:in-theory (enable
+                 ;;                    generic-geval-apply-ev-substitution
+                 ;;                    generic-geval-apply-ev-of-fncall-args)))
+                 ;; (and stable-under-simplificationp
+                 ;;      '(:expand ((generic-geval-ev-concrete-lst
+                 ;;                  acl2::x-lst a appalist)
+                 ;;                 (generic-geval-apply-ev-substitution
+                 ;;                  x a appalist))))
+                 )
+         :rule-classes nil
+         :otf-flg t))
 
 (defun get-guard-verification-theorem (name state)
   (declare (xargs :mode :program
@@ -319,53 +458,124 @@
 (defconst *geval-appalist-func-inst-template*
   '(:computed-hint-replacement
     ((and stable-under-simplificationp
-; (not (cw "clause: ~x0~%" clause))
-          ;; both clauses should be of the form ((equal a b))
-          (if (equal (car (cadr (car clause))) ;; fn symbol of A
-                     '_geval_-appalist)
-              '(:expand ((_geval_-appalist x env appalist))
-                :do-not nil)
-            '(:clause-processor (apply-with-stub/alist-cp clause
-                                                          nil
-                                                          state)))))
-    :use ((:functional-instance
-           _thmname_
-           (_geval_
-            (lambda (x env)
-              (_geval_-appalist x env appalist)))
-           (apply-stub
-            (lambda (f args)
-              (cdr (assoc (cons f args) appalist))))
-           (_geval_-apply
-            (lambda (fn args)
-              (IF (AND (MEMBER-EQUAL (CONS FN (LEN ARGS))
-                                     (_geval_-APPLY-ARITIES))
-                       (TRUE-LISTP ARGS))
-                  (_geval_-APPLY FN ARGS)
-                  (CDR (ASSOC (CONS FN ARGS)
-                              APPALIST)))))))
-    :in-theory nil
-    :do-not '(preprocess simplify)))
+          '(:expand ((:free (f ar)
+                      (_geval_-apply f ar))))))
+    :use
+    ((:functional-instance
+      _theorem_
+      (_geval_ (lambda (x env)
+                       (_geval_-appalist x env appalist)))
+      (_geval_-ev (lambda (x a)
+                          (_geval_-ev-concrete x a appalist)))
+      (_geval_-ev-lst
+       (lambda (x a)
+               (_geval_-ev-concrete-lst x a appalist)))))
+    :in-theory '(nth-of-_geval_-ev-concrete-lst
+                 acl2::car-to-nth-meta-correct
+                 acl2::nth-of-cdr
+                 _geval_-ev-concrete-lst-of-kwote-lst
+                 acl2::list-fix-when-true-listp
+                 acl2::kwote-list-list-fix
+                 (:t _geval_-ev-concrete-lst)
+                 (:t acl2::list-fix)
+                 car-cons cdr-cons nth-0-cons (nfix))
+    :expand ((_geval_-ev-concrete x a appalist)
+             (:free (f ar)
+              (_geval_-ev-concrete (cons f ar) nil appalist))
+             (_geval_-ev-concrete-lst acl2::x-lst a appalist)
+             (_geval_-appalist x env appalist))
+    :do-not-induct t))
+
+
+;; (:use ((:functional-instance
+;;            _geval_
+;;            (_geval_
+;;             (lambda (x env)
+;;               (_geval_-appalist x env appalist)))
+;;            (_geval_-ev
+;;             (lambda (x a)
+;;               (_geval_-ev-concrete x a appalist)))
+;;            (_geval_-ev-lst
+;;             (lambda (x a)
+;;               (_geval_-ev-concrete-lst
+;;                x a appalist)))))
+;;     ;; '(generic-geval-apply-ev-lst-of-atom
+;;     ;;   generic-geval-apply-ev-substitution)
+;;     ;; :in-theory '(generic-geval-apply
+;;     ;;              generic-geval-apply-arities
+;;     ;;              member-equal
+;;     ;;              generic-geval-appalist)
+;;     :do-not-induct t))
+;;   '(:computed-hint-replacement
+;;     ((and stable-under-simplificationp
+;; ; (not (cw "clause: ~x0~%" clause))
+;;           ;; both clauses should be of the form ((equal a b))
+;;           (if (equal (car (cadr (car clause))) ;; fn symbol of A
+;;                      '_geval_-appalist)
+;;               '(:expand ((_geval_-appalist x env appalist))
+;;                 :do-not nil)
+;;             '(:clause-processor (apply-with-stub/alist-cp clause
+;;                                                           nil
+;;                                                           state)))))
+;;     :use ((:functional-instance
+;;            _thmname_
+;;            (_geval_
+;;             (lambda (x env)
+;;               (_geval_-appalist x env appalist)))
+;;            (apply-stub
+;;             (lambda (f args)
+;;               (cdr (assoc (cons f args) appalist))))
+;;            (_geval_-apply
+;;             (lambda (fn args)
+;;               (IF (AND (MEMBER-EQUAL (CONS FN (LEN ARGS))
+;;                                      (_geval_-APPLY-ARITIES))
+;;                        (TRUE-LISTP ARGS))
+;;                   (_geval_-APPLY FN ARGS)
+;;                   (CDR (ASSOC (CONS FN ARGS)
+;;                               APPALIST)))))))
+;;     :in-theory nil
+;;     :do-not '(preprocess simplify)))
 
 (defun geval-appalist-functional-inst-hint (thm geval)
   (declare (xargs :mode :program))
   (acl2::template-subst
    *geval-appalist-func-inst-template*
    :atom-alist `((_geval_ . ,geval)
-                 (_thmname_ . ,thm))
+                 (_theorem_ . ,thm))
    :str-alist `(("_GEVAL_" . ,(symbol-name geval)))
    :pkg-sym geval))
 
 
 (defconst *def-eval-g-template*
   '(progn
+     (local (in-theory #!acl2 (enable car-cdr-elim
+                                      car-cons
+                                      cdr-cons
+                                      acl2-count
+                                      (:t acl2-count)
+                                      o< o-finp
+                                      acl2::true-listp-of-list-fix
+                                      pseudo-term-listp
+                                      pseudo-termp
+                                      eqlablep
+                                      consp-assoc-equal
+                                      assoc-eql-exec-is-assoc-equal
+                                      alistp-pairlis$
+                                      atom not eq
+                                      symbol-listp-forward-to-true-listp)))
      (def-geval _geval_ _apply-fns_)
      (verify-guards _geval_
-       :hints (("goal" :by (:functional-instance
-                            generic-geval-guards-ok
-                            (generic-geval _geval_)
-                            (generic-geval-apply _geval_-apply)
-                            (apply-stub _geval_-apply)))))
+       :hints (("goal" :use ((:functional-instance
+                              generic-geval-guards-ok
+                              (generic-geval _geval_)
+                              (generic-geval-ev _geval_-ev)
+                              (generic-geval-ev-lst _geval_-ev-lst)))
+                :in-theory (e/d* (_geval_-ev-constraint-0
+                                  _geval_-apply-agrees-with-_geval_-ev
+                                  eq atom
+                                  generic-geval-apply)
+                                 (_geval_-apply))))
+       :otf-flg t)
      (local (defthm _geval_-appalist-is-instance-of-_geval_
               t
               :hints ((geval-appalist-functional-inst-hint '_geval_ '_geval_))
@@ -383,6 +593,41 @@
  ;; test
  (def-eval-g implies-geval
    (implies)))
+
+
+
+;; (DEFTHM LITTLE-GEVAL-APPALIST-IS-INSTANCE-OF-LITTLE-GEVAL
+;;   T
+;;   :HINTS ('(:computed-hint-replacement
+;;             ((and stable-under-simplificationp
+;;                   '(:expand ((:free (f ar)
+;;                               (little-geval-apply f ar))))))
+;;             :USE
+;;             ((:FUNCTIONAL-INSTANCE
+;;               LITTLE-GEVAL
+;;               (LITTLE-GEVAL (LAMBDA (X ENV)
+;;                                     (LITTLE-GEVAL-APPALIST X ENV APPALIST)))
+;;               (LITTLE-GEVAL-EV (LAMBDA (X A)
+;;                                        (LITTLE-GEVAL-EV-CONCRETE X A APPALIST)))
+;;               (LITTLE-GEVAL-EV-LST
+;;                (LAMBDA (X A)
+;;                        (LITTLE-GEVAL-EV-CONCRETE-LST X A APPALIST)))))
+;;             :in-theory '(nth-of-little-geval-ev-concrete-lst
+;;                          acl2::car-to-nth-meta-correct
+;;                          acl2::nth-of-cdr
+;;                          little-geval-ev-concrete-lst-of-kwote-lst
+;;                          acl2::list-fix-when-true-listp
+;;                          acl2::kwote-list-list-fix
+;;                          (:t little-geval-ev-concrete-lst)
+;;                          (:t acl2::list-fix)
+;;                          car-cons cdr-cons nth-0-cons (nfix))
+;;             :expand ((little-geval-ev-concrete x a appalist)
+;;                      (:free (f ar)
+;;                       (little-geval-ev-concrete (cons f ar) nil appalist))
+;;                      (little-geval-ev-concrete-lst acl2::x-lst a appalist)
+;;                      (little-geval-appalist x env appalist))
+;;             :DO-NOT-INDUCT T))
+;;   :RULE-CLASSES NIL)
 
 (with-output :off :all :on (error)
   (local
